%\vspace{1ex}
\vspace{0.3ex}
\noindent\textbf{Activity 1.09.1}

%\vspace{0.75ex}
\vspace{0.2ex}

Find the remainder when each polynomial is divided by \( x - c \) using the Remainder Theorem.
\begin{enumerate}
    \item \( f(x) = x^3 - 5x^2 + 7x - 20 \), \( c = 3 \)
    \item \( f(x) = 2x^4 - x^3 + 3x - 7 \), \( c = -2 \)
    \item \( f(x) = x^5 - 2x^3 + x - 9 \), \( c = 2 \)
    \item \( f(x) = 4x^3 + 5x^2 - x + 12 \), \( c = -1 \)
    \item \( f(x) = 5x^4 - 7x^2 + x + 14 \), \( c = -3 \)
    \item \( f(x) = 6x^3 - 2x + 18 \), \( c = 5 \)
    \item \( f(x) = x^4 - 4x^2 + 10 \), \( c = -1 \)
    \item \( f(x) = 3x^5 - x^3 + 6x - 4 \), \( c = 0 \)
    \item \( f(x) = x^6 - 6x^4 + 3x^2 - 2x + 11 \), \( c = -2 \)
    \item \( f(x) = 2x^3 + 3x^2 - 5x + 2 \), \( c = 4 \)
\end{enumerate}