%\vspace{1ex}
\vspace{0.3ex}
\noindent\textbf{Practice Exercises 1.09.1}

%\vspace{0.75ex}
\vspace{0.2ex}

Evaluate the remainder when each polynomial is divided by \( x - c \) using the Remainder Theorem.
\begin{enumerate}
    \item \( f(x) = x^3 - 4x^2 + 6x - 24 \), \( c = 2 \)
    \item \( f(x) = 2x^4 - 3x^3 + x - 5 \), \( c = -1 \)
    \item \( f(x) = x^5 - x^3 + 2x - 8 \), \( c = 1 \)
    \item \( f(x) = 4x^3 + 7x^2 - 2x + 10 \), \( c = 3 \)
    \item \( f(x) = 5x^4 - 9x^2 + x + 12 \), \( c = -2 \)
    \item \( f(x) = 6x^3 - 4x + 15 \), \( c = 4 \)
    \item \( f(x) = x^4 - 3x^2 + 8 \), \( c = 0 \)
    \item \( f(x) = 3x^5 - 2x^3 + 7x - 6 \), \( c = -3 \)
    \item \( f(x) = x^6 - 5x^4 + 2x^2 - x + 9 \), \( c = 1 \)
    \item \( f(x) = 2x^3 + 4x^2 - 6x + 1 \), \( c = 5 \)
\end{enumerate}