%\vspace{1ex}
\vspace{0.3ex}
\noindent\textbf{Activity 1.09.2}

%\vspace{0.75ex}
\vspace{0.2ex}

\begin{enumerate}
    \item Use the Factor Theorem to determine if \( (x - 3) \) is a factor of \( P(x) = x^3 - 5x^2 + 8x - 6 \).
    \item Check whether \( (x + 2) \) is a factor of \( P(x) = x^3 + 5x^2 + 8x + 4 \).
    \item Determine if \( (x - 6) \) is a factor of \( P(x) = x^4 - 6x^3 + 12x^2 - 36x + 36 \).
    \item Verify if \( (x + 4) \) is a factor of \( P(x) = x^3 + 3x^2 - 2x - 12 \).
    \item Use the Factor Theorem to check if \( (x - 7) \) is a factor of \( P(x) = x^3 - 9x^2 + 21x - 14 \).
    \item Test whether \( (x - 5) \) is a factor of \( P(x) = x^3 - 10x^2 + 25x - 25 \).
    \item Is \( (x + 3) \) a factor of \( P(x) = x^4 + 6x^3 + 9x^2 - 9x - 27 \)?
    \item Check if \( (x - 2) \) is a factor of \( P(x) = x^5 - 2x^4 + 2x^3 - 2x^2 + 2x - 2 \).
    \item Verify whether \( (x + 6) \) is a factor of \( P(x) = x^3 + 18x^2 + 108x + 216 \).
    \item Use the Factor Theorem to test if \( (x - 4) \) is a factor of \( P(x) = x^3 - 8x^2 + 17x - 12 \).
\end{enumerate}