%\vspace{1ex}
\vspace{0.3ex}
\noindent\textbf{Practice Exercises 1.09.2}

%\vspace{0.75ex}
\vspace{0.2ex}

\begin{enumerate}
    \item Use the Factor Theorem to determine if \( (x - 2) \) is a factor of \( P(x) = x^3 - 4x^2 + 5x - 2 \).
    \item Check whether \( (x + 3) \) is a factor of \( P(x) = x^3 + 6x^2 + 11x + 6 \).
    \item Determine if \( (x - 5) \) is a factor of \( P(x) = x^4 - 5x^3 + 10x^2 - 25x + 25 \).
    \item Verify if \( (x + 1) \) is a factor of \( P(x) = x^3 + 2x^2 - x - 2 \).
    \item Use the Factor Theorem to check if \( (x - 4) \) is a factor of \( P(x) = x^3 - 7x^2 + 14x - 8 \).
    \item Test whether \( (x - 6) \) is a factor of \( P(x) = x^3 - 9x^2 + 27x - 27 \).
    \item Is \( (x + 2) \) a factor of \( P(x) = x^4 + 4x^3 + 4x^2 - 4x - 8 \)?
    \item Check if \( (x - 1) \) is a factor of \( P(x) = x^5 - x^4 + x^3 - x^2 + x - 1 \).
    \item Verify whether \( (x + 5) \) is a factor of \( P(x) = x^3 + 15x^2 + 75x + 125 \).
    \item Use the Factor Theorem to test if \( (x - 3) \) is a factor of \( P(x) = x^3 - 6x^2 + 11x - 6 \).
\end{enumerate}