\vspace{1ex}
\noindent\textbf{Activity 1.1.1}

\vspace{0.75ex}
 
%\vspace{-1ex}
%\begin{multicols}{2}
\begin{enumerate}[label = \color{blue} \Alph*. ]
%1		
   \item Determine whether each equation is quadratic or not quadratic.
   %\vspace{-1ex}
\begin{multicols}{3}
\begin{enumerate}[label = \color{blue}\arabic*. ] 
%1
   \item $ 2(x + 3) = 0 $
%2
   \item $ x + 3x^2 = 0 $
%3
   \item $ 5x - 4 = 0 $
%4
   \item $ -2m^2 + m = 1 $
%5
   \item $ (t + 4)(t+7) = 0 $
\end{enumerate}
\end{multicols}
				 
   \item Express the following in standard form, then determine the values of $a$, $b$, and $c$.
   %\vspace{-1ex}
\begin{multicols}{3}
\begin{enumerate}[label = \color{blue} \arabic*. ]
%1
   \item $ x^2 - 6x - 7 = 0 $

%2
   \item $ x^2 - 64 = 0 $
%3
   \item $ -2x +8 = -9x^2 $
%4
   \item $ x^2 = 3x + 10 $
%5
   \item $ 4x^2 - 2 = 0 $
\end{enumerate}
\end{multicols}
		 
   \item Express the following in the standard form and identify the quadratic term, linear term, and constant term.
%\vspace{-1ex}
\begin{multicols}{2}
\begin{enumerate}[label = \color{blue}\arabic*. ]
%1
   \item $ 2x(x + 1) = 0 $

%2
   \item $ (x + 4)^2 = 5 $
%3
   \item $ (x + 3)(x - 3) = x(4x + 5) $
%4
   \item $ (x + 5)(x - 9) = 21 $
%5
   \item $ x(2x - 4) = (x - 2)(x - 2) $ 
\end{enumerate}
\end{multicols}
	 
\end{enumerate}
%\end{multicols}
				
				
