%\vspace{1ex}
\vspace{0.3ex}
\noindent\textbf{Activity 2.31}

%\vspace{0.75ex}
\vspace{0.2ex}

Transform the given equation to its other form.

\begin{enumerate}
    \item Convert $(x - 3)^2 + (y + 2)^2 = 25$ to general form.
%    \item Convert $(x + 4)^2 + (y - 1)^2 = 36$ to general form.
    \item Convert $(x - 2)^2 + (y - 5)^2 = 49$ to general form.
   % \item Convert $(x + 5)^2 + (y + 3)^2 = 64$ to general form.
    \item Convert $x^2 + y^2 - 6x + 8y - 11 = 0$ to center-radius form.
    %\item Convert $x^2 + y^2 + 10x - 4y - 7 = 0$ to center-radius form.
    \item Convert $x^2 + y^2 - 2x + 12y + 30 = 0$ to center-radius form.
    %\item Convert $(x - 1)^2 + (y + 7)^2 = 81$ to general form.
    \item Convert $x^2 + y^2 + 14x - 6y + 20 = 0$ to center-radius form.
    %\item Convert $(x + 6)^2 + (y - 2)^2 = 100$ to general form.
\end{enumerate}
