%\vspace{1ex}
\vspace{0.3ex}
\noindent\textbf{Practice Exercises 2.31}

%\vspace{0.75ex}
\vspace{0.2ex}

Transform the given equation to its other form.

\begin{enumerate}
 %   \item Convert $(x - 4)^2 + (y + 3)^2 = 16$ to general form.
    \item Convert $(x + 5)^2 + (y - 2)^2 = 49$ to general form.
    %\item Convert $(x - 3)^2 + (y - 6)^2 = 64$ to general form.
    \item Convert $(x + 6)^2 + (y + 4)^2 = 81$ to general form.
    %\item Convert $x^2 + y^2 - 8x + 6y - 15 = 0$ to center-radius form.
    \item Convert $x^2 + y^2 + 12x - 2y - 5 = 0$ to center-radius form.
    %\item Convert $x^2 + y^2 - 4x + 10y + 35 = 0$ to center-radius form.
    \item Convert $(x - 2)^2 + (y + 6)^2 = 49$ to general form.
    %\item Convert $x^2 + y^2 + 16x - 8y + 24 = 0$ to center-radius form.
    \item Convert $(x + 7)^2 + (y - 3)^2 = 121$ to general form.
\end{enumerate}
